Create standalone class for term_meta.

crypto.v
@@ -793,70 +793,81 @@ Lemma pterm_TEncIP k t :
   pterm (TEnc k t).
 Proof. by iIntros "? ?"; rewrite pterm_TEnc; eauto. Qed.
 
-Section Meta.
+Section TermMeta.
 
-Context `{!EqDecision L, !Countable L}.
+Context (term_meta : ∀ `{Countable L}, term → namespace → L → iProp).
+Context (term_meta_token : term → coPset → iProp).
+
+Class TermMeta := {
+  term_meta_persistent :> ∀ `{Countable L} t N (x : L),
+    Persistent (term_meta _ t N x);
+  term_meta_set : ∀ `{Countable L} E t (x : L) N,
+    ↑N ⊆ E →
+    term_meta_token t E ==∗ term_meta _ t N x;
+  term_meta_meta_token : ∀ `{Countable L} t (x : L) N E,
+    ↑N ⊆ E →
+    term_meta_token t E -∗ term_meta _ t N x -∗ False;
+  term_meta_agree : ∀ `{Countable L} t N (x1 x2 : L),
+    term_meta _ t N x1 -∗
+    term_meta _ t N x2 -∗
+    ⌜x1 = x2⌝;
+  term_meta_token_difference : ∀ t (E1 E2 : coPset),
+    E1 ⊆ E2 →
+    term_meta_token t E2 ⊣⊢
+    term_meta_token t E1 ∗ term_meta_token t (E2 ∖ E1);
+}.
+
+End TermMeta.
 
 (* Using two locations is a bit ugly, but maybe more convenient *)
 
-Definition term_meta_token t E : iProp :=
-  match t with
-  | TNonce a => ∃ a', meta a (nroot.@"meta") a' ∧ meta_token a' E
-  | _ => False
-  end.
-
-Definition term_meta t N (x : L) : iProp :=
+Definition nonce_meta `{Countable L} t N (x : L) : iProp :=
   match t with
   | TNonce a => ∃ a', meta a (nroot.@"meta") a' ∧ meta a' N x
   | _ => False
   end.
 
-Global Instance persistent_term_meta t N x :
-  Persistent (term_meta t N x).
-Proof. case: t => *; apply _. Qed.
+Definition nonce_meta_token t E : iProp :=
+  match t with
+  | TNonce a => ∃ a', meta a (nroot.@"meta") a' ∧ meta_token a' E
+  | _ => False
+  end.
 
-Lemma term_meta_set t N E x :
-  ↑N ⊆ E → term_meta_token t E ==∗ term_meta t N x.
-Proof.
-case: t; try by move=> *; iStartProof.
+Program Global Instance nonce_term_meta :
+  TermMeta (@nonce_meta) nonce_meta_token.
+
+Next Obligation. move=> ???; case=> *; apply _. Qed.
+
+Next Obligation.
+move=> ??? E t x N; case: t; try by move=> *; iStartProof.
 move=> a; iIntros (sub) "token"; rewrite /=.
 iDestruct "token" as (a') "[meta_a' token]".
 by iMod (meta_set E _ x with "token") as "meta"; eauto.
 Qed.
 
-Lemma term_meta_meta_token t (x : L) N E :
-  ↑N ⊆ E → term_meta_token t E -∗ term_meta t N x -∗ False.
-Proof.
-case: t; try by move=> *; iStartProof.
-move=> a sub /=; iIntros "token meta".
+Next Obligation.
+move=> ???; case; try by move=> *; iStartProof.
+move=> a x N E sub /=; iIntros "token meta".
 iDestruct "token" as (a1) "[meta_a1 token]".
 iDestruct "meta"  as (a2) "[meta_a2 meta]".
 iPoseProof (meta_agree with "meta_a1 meta_a2") as "->".
 by iDestruct (meta_meta_token with "token meta") as "[]".
 Qed.
 
-Lemma term_meta_agree t N (x1 x2 : L) :
-  term_meta t N x1 -∗
-  term_meta t N x2 -∗
-  ⌜x1 = x2⌝.
-Proof.
-case: t; try by move=> *; iStartProof.
-move=> a /=; iIntros "meta1 meta2".
+Next Obligation.
+move=> ???; case; try by move=> *; iStartProof.
+move=> a * /=; iIntros "meta1 meta2".
 iDestruct "meta1" as (a1) "[meta_a1 meta1]".
 iDestruct "meta2" as (a2) "[meta_a2 meta2]".
 iPoseProof (meta_agree with "meta_a1 meta_a2") as "->".
 by iApply (meta_agree with "meta1 meta2").
 Qed.
 
-Lemma term_meta_token_difference t E1 E2 :
-  E1 ⊆ E2 →
-  term_meta_token t E2 ⊣⊢
-  term_meta_token t E1 ∗ term_meta_token t (E2 ∖ E1).
-Proof.
-case: t; try by move=> *; iSplit; [iIntros "[]"|iIntros "[[] ?]"].
-move=> a sub; iSplit.
+Next Obligation.
+case; try by move=> *; iSplit; [iIntros "[]"|iIntros "[[] ?]"].
+move=> a ?? sub; iSplit.
 - iDestruct 1 as (a') "[#meta_a' token]".
-  rewrite meta_token_difference; eauto.
+  rewrite meta_token_difference /=; eauto.
   iDestruct "token" as "[token1 token2]".
   by iSplitL "token1"; iExists a'; eauto.
 - iDestruct 1 as "[token1 token2]".
@@ -867,8 +878,6 @@ move=> a sub; iSplit.
   by iApply meta_token_difference => //; iSplitL "token1".
 Qed.
 
-End Meta.
-
 End Resources.
 
 Arguments crypto_enc_name {Σ _}.
@@ -877,5 +886,6 @@ Arguments crypto_hash_name {Σ _}.
 Arguments hash_pred {Σ _ _}.
 Arguments crypto_key_name {Σ _}.
 Arguments key_pred {Σ _ _}.
-Arguments term_meta_set {Σ _ _ _ _} t N E x.
-Arguments term_meta_token_difference {Σ _} t E1 E2.
+Arguments term_meta_set {Σ _ _ _ _ _ _} E t x N.
+Arguments term_meta_token_difference {Σ _ _ _} t E1 E2.
+Arguments nonce_term_meta Σ {_}.
